Wolfram: make GC causal graph choice-free
Refactors CausalGraphGC to use list-indexed observable events (no Finset.orderIsoOfFin / no Classical.choice), updates CE1/CE2 GC invariance proofs, and refreshes the Wolfram researcher bundle reports + hashed artifacts.

RESEARCHER_BUNDLE/artifacts/compiler/ir/HeytingLean/WPP/Wolfram/CausalGraphGC.c
@@ -1,6 +1,6 @@
 // Lean compiler output
 // Module: HeytingLean.WPP.Wolfram.CausalGraphGC
-// Imports: Init Mathlib.Data.Finset.Sort HeytingLean.WPP.Wolfram.CausalGraph
+// Imports: Init Mathlib.Data.Multiset.Fold HeytingLean.WPP.Wolfram.CausalGraph
 #include <lean/lean.h>
 #if defined(__clang__)
 #pragma clang diagnostic ignored "-Wunused-parameter"
@@ -13,8 +13,216 @@
 #ifdef __cplusplus
 extern "C" {
 #endif
+lean_object* l_HeytingLean_WPP_Wolfram_System_Event_output___redArg(lean_object*, lean_object*);
+LEAN_EXPORT lean_object* l_HeytingLean_WPP_Wolfram_System_causalGraphGCOf(lean_object*, lean_object*, lean_object*, lean_object*, lean_object*, lean_object*);
+lean_object* l_List_lengthTR___redArg(lean_object*);
+lean_object* l_HeytingLean_WPP_Wolfram_System_Event_input___redArg(lean_object*, lean_object*);
+lean_object* l_Multiset_map___redArg(lean_object*, lean_object*);
+LEAN_EXPORT lean_object* l_HeytingLean_WPP_Wolfram_System_observableIdxs(lean_object*, lean_object*, lean_object*, lean_object*, lean_object*, lean_object*);
+LEAN_EXPORT uint8_t l_HeytingLean_WPP_Wolfram_System_Event_observableB___redArg___lam__1(uint8_t, uint8_t);
+LEAN_EXPORT lean_object* l_HeytingLean_WPP_Wolfram_System_Event_observableB___redArg___lam__1___boxed(lean_object*, lean_object*);
+LEAN_EXPORT uint8_t l_HeytingLean_WPP_Wolfram_System_Event_observableB___redArg___lam__0(lean_object*, lean_object*, lean_object*);
+lean_object* l_List_filterTR_loop___redArg(lean_object*, lean_object*, lean_object*);
+LEAN_EXPORT lean_object* l_HeytingLean_WPP_Wolfram_System_Event_observableB___redArg___lam__2___boxed(lean_object*, lean_object*, lean_object*, lean_object*, lean_object*, lean_object*);
+uint8_t l_List_hasDecEq___redArg(lean_object*, lean_object*, lean_object*);
+LEAN_EXPORT lean_object* l_HeytingLean_WPP_Wolfram_System_causalGraphGCOf___redArg(lean_object*, lean_object*, lean_object*, lean_object*);
+LEAN_EXPORT lean_object* l_HeytingLean_WPP_Wolfram_System_observableIdxs___redArg___lam__0___boxed(lean_object*, lean_object*, lean_object*, lean_object*, lean_object*);
+LEAN_EXPORT lean_object* l_HeytingLean_WPP_Wolfram_System_Event_observableB___boxed(lean_object*, lean_object*, lean_object*, lean_object*, lean_object*, lean_object*);
+lean_object* l_List_foldrTR___redArg(lean_object*, lean_object*, lean_object*);
+LEAN_EXPORT lean_object* l_HeytingLean_WPP_Wolfram_System_Event_observableB___redArg___lam__0___boxed(lean_object*, lean_object*, lean_object*);
+lean_object* l_List_get___redArg(lean_object*, lean_object*);
+LEAN_EXPORT uint8_t l_HeytingLean_WPP_Wolfram_System_observableIdxs___redArg___lam__0(lean_object*, lean_object*, lean_object*, lean_object*, lean_object*);
+uint8_t l_Multiset_decidableMem___redArg(lean_object*, lean_object*, lean_object*);
+uint8_t l_instDecidableNot___redArg(uint8_t);
+LEAN_EXPORT uint8_t l_HeytingLean_WPP_Wolfram_System_Event_observableB___redArg___lam__2(lean_object*, lean_object*, lean_object*, lean_object*, lean_object*, lean_object*);
+lean_object* l_List_finRange(lean_object*);
+LEAN_EXPORT uint8_t l_HeytingLean_WPP_Wolfram_System_Event_observableB(lean_object*, lean_object*, lean_object*, lean_object*, lean_object*, lean_object*);
+LEAN_EXPORT lean_object* l_HeytingLean_WPP_Wolfram_System_observableIdxs___redArg(lean_object*, lean_object*, lean_object*, lean_object*);
+LEAN_EXPORT lean_object* l_HeytingLean_WPP_Wolfram_System_Event_observableB___redArg(lean_object*, lean_object*, lean_object*, lean_object*);
+LEAN_EXPORT uint8_t l_HeytingLean_WPP_Wolfram_System_Event_observableB___redArg___lam__0(lean_object* x_1, lean_object* x_2, lean_object* x_3) {
+_start:
+{
+uint8_t x_4; 
+x_4 = l_List_hasDecEq___redArg(x_1, x_2, x_3);
+return x_4;
+}
+}
+LEAN_EXPORT uint8_t l_HeytingLean_WPP_Wolfram_System_Event_observableB___redArg___lam__2(lean_object* x_1, lean_object* x_2, lean_object* x_3, lean_object* x_4, lean_object* x_5, lean_object* x_6) {
+_start:
+{
+lean_object* x_7; uint8_t x_8; uint8_t x_9; 
+x_7 = l_HeytingLean_WPP_Wolfram_System_Event_input___redArg(x_1, x_2);
+lean_inc(x_6);
+x_8 = l_Multiset_decidableMem___redArg(x_3, x_6, x_7);
+x_9 = l_instDecidableNot___redArg(x_8);
+if (x_9 == 0)
+{
+lean_dec(x_6);
+lean_dec(x_5);
+lean_dec_ref(x_4);
+return x_9;
+}
+else
+{
+uint8_t x_10; 
+x_10 = l_Multiset_decidableMem___redArg(x_4, x_6, x_5);
+return x_10;
+}
+}
+}
+LEAN_EXPORT uint8_t l_HeytingLean_WPP_Wolfram_System_Event_observableB___redArg___lam__1(uint8_t x_1, uint8_t x_2) {
+_start:
+{
+if (x_1 == 0)
+{
+return x_2;
+}
+else
+{
+return x_1;
+}
+}
+}
+LEAN_EXPORT lean_object* l_HeytingLean_WPP_Wolfram_System_Event_observableB___redArg(lean_object* x_1, lean_object* x_2, lean_object* x_3, lean_object* x_4) {
+_start:
+{
+lean_object* x_5; lean_object* x_6; lean_object* x_7; uint8_t x_8; lean_object* x_9; lean_object* x_10; lean_object* x_11; lean_object* x_12; 
+x_5 = lean_alloc_closure((void*)(l_HeytingLean_WPP_Wolfram_System_Event_observableB___redArg___lam__0___boxed), 3, 1);
+lean_closure_set(x_5, 0, x_2);
+lean_inc_ref(x_5);
+lean_inc_ref(x_3);
+lean_inc_ref(x_1);
+x_6 = lean_alloc_closure((void*)(l_HeytingLean_WPP_Wolfram_System_Event_observableB___redArg___lam__2___boxed), 6, 5);
+lean_closure_set(x_6, 0, x_1);
+lean_closure_set(x_6, 1, x_3);
+lean_closure_set(x_6, 2, x_5);
+lean_closure_set(x_6, 3, x_5);
+lean_closure_set(x_6, 4, x_4);
+x_7 = lean_alloc_closure((void*)(l_HeytingLean_WPP_Wolfram_System_Event_observableB___redArg___lam__1___boxed), 2, 0);
+x_8 = 0;
+x_9 = l_HeytingLean_WPP_Wolfram_System_Event_output___redArg(x_1, x_3);
+lean_dec_ref(x_1);
+x_10 = l_Multiset_map___redArg(x_6, x_9);
+x_11 = lean_box(x_8);
+x_12 = l_List_foldrTR___redArg(x_7, x_11, x_10);
+return x_12;
+}
+}
+LEAN_EXPORT uint8_t l_HeytingLean_WPP_Wolfram_System_Event_observableB(lean_object* x_1, lean_object* x_2, lean_object* x_3, lean_object* x_4, lean_object* x_5, lean_object* x_6) {
+_start:
+{
+lean_object* x_7; uint8_t x_8; 
+x_7 = l_HeytingLean_WPP_Wolfram_System_Event_observableB___redArg(x_3, x_4, x_5, x_6);
+x_8 = lean_unbox(x_7);
+lean_dec(x_7);
+return x_8;
+}
+}
+LEAN_EXPORT lean_object* l_HeytingLean_WPP_Wolfram_System_Event_observableB___redArg___lam__0___boxed(lean_object* x_1, lean_object* x_2, lean_object* x_3) {
+_start:
+{
+uint8_t x_4; lean_object* x_5; 
+x_4 = l_HeytingLean_WPP_Wolfram_System_Event_observableB___redArg___lam__0(x_1, x_2, x_3);
+x_5 = lean_box(x_4);
+return x_5;
+}
+}
+LEAN_EXPORT lean_object* l_HeytingLean_WPP_Wolfram_System_Event_observableB___redArg___lam__2___boxed(lean_object* x_1, lean_object* x_2, lean_object* x_3, lean_object* x_4, lean_object* x_5, lean_object* x_6) {
+_start:
+{
+uint8_t x_7; lean_object* x_8; 
+x_7 = l_HeytingLean_WPP_Wolfram_System_Event_observableB___redArg___lam__2(x_1, x_2, x_3, x_4, x_5, x_6);
+lean_dec_ref(x_1);
+x_8 = lean_box(x_7);
+return x_8;
+}
+}
+LEAN_EXPORT lean_object* l_HeytingLean_WPP_Wolfram_System_Event_observableB___redArg___lam__1___boxed(lean_object* x_1, lean_object* x_2) {
+_start:
+{
+uint8_t x_3; uint8_t x_4; uint8_t x_5; lean_object* x_6; 
+x_3 = lean_unbox(x_1);
+x_4 = lean_unbox(x_2);
+x_5 = l_HeytingLean_WPP_Wolfram_System_Event_observableB___redArg___lam__1(x_3, x_4);
+x_6 = lean_box(x_5);
+return x_6;
+}
+}
+LEAN_EXPORT lean_object* l_HeytingLean_WPP_Wolfram_System_Event_observableB___boxed(lean_object* x_1, lean_object* x_2, lean_object* x_3, lean_object* x_4, lean_object* x_5, lean_object* x_6) {
+_start:
+{
+uint8_t x_7; lean_object* x_8; 
+x_7 = l_HeytingLean_WPP_Wolfram_System_Event_observableB(x_1, x_2, x_3, x_4, x_5, x_6);
+x_8 = lean_box(x_7);
+return x_8;
+}
+}
+LEAN_EXPORT uint8_t l_HeytingLean_WPP_Wolfram_System_observableIdxs___redArg___lam__0(lean_object* x_1, lean_object* x_2, lean_object* x_3, lean_object* x_4, lean_object* x_5) {
+_start:
+{
+lean_object* x_6; lean_object* x_7; uint8_t x_8; 
+x_6 = l_List_get___redArg(x_1, x_5);
+x_7 = l_HeytingLean_WPP_Wolfram_System_Event_observableB___redArg(x_2, x_3, x_6, x_4);
+x_8 = lean_unbox(x_7);
+return x_8;
+}
+}
+LEAN_EXPORT lean_object* l_HeytingLean_WPP_Wolfram_System_observableIdxs___redArg(lean_object* x_1, lean_object* x_2, lean_object* x_3, lean_object* x_4) {
+_start:
+{
+lean_object* x_5; lean_object* x_6; lean_object* x_7; lean_object* x_8; lean_object* x_9; 
+lean_inc(x_3);
+x_5 = lean_alloc_closure((void*)(l_HeytingLean_WPP_Wolfram_System_observableIdxs___redArg___lam__0___boxed), 5, 4);
+lean_closure_set(x_5, 0, x_3);
+lean_closure_set(x_5, 1, x_1);
+lean_closure_set(x_5, 2, x_2);
+lean_closure_set(x_5, 3, x_4);
+x_6 = l_List_lengthTR___redArg(x_3);
+lean_dec(x_3);
+x_7 = l_List_finRange(x_6);
+x_8 = lean_box(0);
+x_9 = l_List_filterTR_loop___redArg(x_5, x_7, x_8);
+return x_9;
+}
+}
+LEAN_EXPORT lean_object* l_HeytingLean_WPP_Wolfram_System_observableIdxs(lean_object* x_1, lean_object* x_2, lean_object* x_3, lean_object* x_4, lean_object* x_5, lean_object* x_6) {
+_start:
+{
+lean_object* x_7; 
+x_7 = l_HeytingLean_WPP_Wolfram_System_observableIdxs___redArg(x_3, x_4, x_5, x_6);
+return x_7;
+}
+}
+LEAN_EXPORT lean_object* l_HeytingLean_WPP_Wolfram_System_observableIdxs___redArg___lam__0___boxed(lean_object* x_1, lean_object* x_2, lean_object* x_3, lean_object* x_4, lean_object* x_5) {
+_start:
+{
+uint8_t x_6; lean_object* x_7; 
+x_6 = l_HeytingLean_WPP_Wolfram_System_observableIdxs___redArg___lam__0(x_1, x_2, x_3, x_4, x_5);
+lean_dec(x_1);
+x_7 = lean_box(x_6);
+return x_7;
+}
+}
+LEAN_EXPORT lean_object* l_HeytingLean_WPP_Wolfram_System_causalGraphGCOf___redArg(lean_object* x_1, lean_object* x_2, lean_object* x_3, lean_object* x_4) {
+_start:
+{
+lean_object* x_5; lean_object* x_6; 
+x_5 = l_HeytingLean_WPP_Wolfram_System_observableIdxs___redArg(x_1, x_2, x_3, x_4);
+x_6 = l_List_lengthTR___redArg(x_5);
+lean_dec(x_5);
+return x_6;
+}
+}
+LEAN_EXPORT lean_object* l_HeytingLean_WPP_Wolfram_System_causalGraphGCOf(lean_object* x_1, lean_object* x_2, lean_object* x_3, lean_object* x_4, lean_object* x_5, lean_object* x_6) {
+_start:
+{
+lean_object* x_7; 
+x_7 = l_HeytingLean_WPP_Wolfram_System_causalGraphGCOf___redArg(x_3, x_4, x_5, x_6);
+return x_7;
+}
+}
 lean_object* initialize_Init(uint8_t builtin, lean_object*);
-lean_object* initialize_Mathlib_Data_Finset_Sort(uint8_t builtin, lean_object*);
+lean_object* initialize_Mathlib_Data_Multiset_Fold(uint8_t builtin, lean_object*);
 lean_object* initialize_HeytingLean_WPP_Wolfram_CausalGraph(uint8_t builtin, lean_object*);
 static bool _G_initialized = false;
 LEAN_EXPORT lean_object* initialize_HeytingLean_WPP_Wolfram_CausalGraphGC(uint8_t builtin, lean_object* w) {
@@ -24,7 +232,7 @@ _G_initialized = true;
 res = initialize_Init(builtin, lean_io_mk_world());
 if (lean_io_result_is_error(res)) return res;
 lean_dec_ref(res);
-res = initialize_Mathlib_Data_Finset_Sort(builtin, lean_io_mk_world());
+res = initialize_Mathlib_Data_Multiset_Fold(builtin, lean_io_mk_world());
 if (lean_io_result_is_error(res)) return res;
 lean_dec_ref(res);
 res = initialize_HeytingLean_WPP_Wolfram_CausalGraph(builtin, lean_io_mk_world());
